Logic/Propositional/Basic/Completeness.lean
@@ -1,0 +1,205 @@
+import Logic.AutoProver.Prover
+import Logic.Propositional.Basic.Semantics
+import Logic.Propositional.Basic.Calculus
+
+namespace LO
+
+namespace Propositional
+
+variable {α : Type*} {Δ : Sequent α}
+
+namespace Sequent
+
+def complexity (Δ : Sequent α) : ℕ := (Δ.map Formula.complexity).sum
+
+end Sequent
+
+namespace Derivation
+
+theorem sound : ⊢¹ Δ → Semantics.Valid Δ.disj := by
+  intro d v
+  induction d
+  case axL Δ a =>
+    simp[List.map_disj]
+    by_cases v a <;> simp[*]
+  case verum => simp[List.map_disj]
+  case and Δ p q _ _ ihp ihq =>
+    by_cases hv : v ⊧ Δ.disj
+    · simp[hv]
+    · have : v ⊧ p := by simpa[hv] using ihp
+      have : v ⊧ q := by simpa[hv] using ihq
+      simp[*]
+  case or Δ p q d ih =>
+    simpa[or_assoc] using ih
+  case wk Δ Γ _ ss ih =>
+    have : ∃ p ∈ Δ, v ⊧ p := by simpa [List.map_disj] using ih
+    rcases this with ⟨p, hp, hvp⟩
+    simp [List.map_disj]; exact ⟨p, ss hp, hvp⟩
+  case cut Δ p _ _ ihp ihn =>
+    by_cases hv : v ⊧ Δ.disj
+    · simp[hv]
+    · have : v ⊧ p := by simpa[hv] using ihp
+      have : ¬v ⊧ p := by simpa[hv] using ihn
+      contradiction
+
+end Derivation
+
+instance : Sound (Formula α) := ⟨by
+  rintro T p ⟨Γ, hΓ, d⟩ v hT
+  by_contra hv
+  have : ∀ v, v ⊧ p ∨ ∃ q ∈ Γ, ¬v ⊧ q := by
+    simpa [Semantics.Valid, List.map_disj] using Derivation.sound (Tait.ofConsRight d)
+  have : ∃ q ∈ Γ, ¬v ⊧ q := by simpa [hv] using this v
+  rcases this with ⟨q, hqΓ, hq⟩
+  have : v ⊧ q := hT (hΓ q hqΓ)
+  contradiction⟩
+
+section complete
+
+def consistentTheory : Set (Theory α) := { U : Theory α | System.Consistent U }
+
+variable {T : Theory α} (consisT : Consistent T)
+open System Gentzen
+
+lemma Set.subset_mem_chain_of_finite (c : Set (Set α)) (hc : Set.Nonempty c) (hchain : IsChain (· ⊆ ·) c)
+    {s} (hfin : Set.Finite s) : s ⊆ ⋃₀ c → ∃ t ∈ c, s ⊆ t :=
+  Set.Finite.induction_on hfin
+    (by rcases hc with ⟨t, ht⟩; intro; exact ⟨t, ht, by simp⟩)
+    (by intro a s _ _ ih h
+        have : ∃ t ∈ c, s ⊆ t := ih (subset_trans (Set.subset_insert a s) h)
+        rcases this with ⟨t, htc, ht⟩
+        have : ∃ u ∈ c, a ∈ u := by simp [Set.insert_subset_iff] at h; exact h.1
+        rcases this with ⟨u, huc, hu⟩
+        have : ∃ z ∈ c, t ⊆ z ∧ u ⊆ z := IsChain.directedOn hchain t htc u huc
+        rcases this with ⟨z, hzc, htz, huz⟩
+        exact ⟨z, hzc, Set.insert_subset (huz hu) (Set.Subset.trans ht htz)⟩)
+
+lemma exists_maximal_consistent_theory :
+    ∃ T', Consistent T' ∧ T ⊆ T' ∧ ∀ U, Consistent U → T' ⊆ U → U = T' :=
+  zorn_subset_nonempty { U : Theory α | Consistent U }
+    (fun c hc chain hnc ↦ ⟨⋃₀ c,
+     by simp
+        by_contra A
+        rcases compact_inconsistent A with ⟨s, hs, s_consis⟩
+        rcases Set.subset_mem_chain_of_finite c hnc chain (s := s) (Finset.finite_toSet s) hs with ⟨U, hUc, hsU⟩
+        have : Consistent (s : Set (Formula α)) := Consistent.of_subset (hc hUc) hsU
+        contradiction,
+     fun s a => Set.subset_sUnion_of_mem a⟩) T consisT
+
+noncomputable def maximalConsistentTheory : Theory α :=
+  Classical.choose (exists_maximal_consistent_theory consisT)
+
+variable {consisT}
+
+@[simp] lemma maximalConsistentTheory_consistent : Consistent (maximalConsistentTheory consisT) :=
+  (Classical.choose_spec (exists_maximal_consistent_theory consisT)).1
+
+@[simp] lemma subset_maximalConsistentTheory : T ⊆ maximalConsistentTheory consisT :=
+  (Classical.choose_spec (exists_maximal_consistent_theory consisT)).2.1
+
+lemma maximalConsistentTheory_maximal :
+    ∀ U, Consistent U → maximalConsistentTheory consisT ⊆ U → U = maximalConsistentTheory consisT :=
+  (Classical.choose_spec (exists_maximal_consistent_theory consisT)).2.2
+
+@[simp] lemma theory_maximalConsistentTheory_eq :
+    theory (maximalConsistentTheory consisT) = maximalConsistentTheory consisT :=
+  maximalConsistentTheory_maximal _ (by simp) (by simp)
+
+lemma mem_or_neg_mem_maximalConsistentTheory (p) :
+    p ∈ maximalConsistentTheory consisT ∨ ~p ∈ maximalConsistentTheory consisT := by
+  by_contra A
+  have hp : p ∉ maximalConsistentTheory consisT ∧ ~p ∉ maximalConsistentTheory consisT := by simpa [not_or] using A
+  have : Consistent (insert p (maximalConsistentTheory consisT)) :=
+    consistent_insert_iff_not_refutable.mpr
+      (unprovable_iff_not_provable.mpr <|
+        show ~p ∉ theory (maximalConsistentTheory consisT) from by simp[hp])
+  have : insert p (maximalConsistentTheory consisT) ≠ maximalConsistentTheory consisT := by
+    simp[hp]
+  have : insert p (maximalConsistentTheory consisT) = maximalConsistentTheory consisT :=
+    maximalConsistentTheory_maximal _ (by assumption) (by simp)
+  contradiction
+
+lemma mem_maximalConsistentTheory_iff :
+    p ∈ maximalConsistentTheory consisT ↔ maximalConsistentTheory consisT ⊢! p :=
+  ⟨fun h ↦ ⟨axm h⟩, fun h ↦ by have : p ∈ theory (maximalConsistentTheory consisT) := h; simpa using this⟩
+
+lemma maximalConsistentTheory_consistent' {p} :
+    p ∈ maximalConsistentTheory consisT → ~p ∉ maximalConsistentTheory consisT := by
+  intro h hn
+  have : ¬Consistent (maximalConsistentTheory consisT) :=
+    inconsistent_of_provable
+      (by prover [mem_maximalConsistentTheory_iff.mp h, mem_maximalConsistentTheory_iff.mp hn])
+  simp_all
+
+lemma not_mem_maximalConsistentTheory_iff :
+    p ∉ maximalConsistentTheory consisT ↔ maximalConsistentTheory consisT ⊢! ~p := by
+  by_cases hp : p ∈ maximalConsistentTheory consisT <;> simp[hp]
+  · apply unprovable_iff_not_provable.mpr
+    intro bnp
+    have : ¬Consistent (maximalConsistentTheory consisT) :=
+      inconsistent_of_provable (by prover [mem_maximalConsistentTheory_iff.mp hp, bnp])
+    simp_all
+  · exact mem_maximalConsistentTheory_iff.mp
+      (by simpa [hp] using mem_or_neg_mem_maximalConsistentTheory (consisT := consisT) p)
+
+lemma mem_maximalConsistentTheory_and {p q} (h : p ⋏ q ∈ maximalConsistentTheory consisT) :
+    p ∈ maximalConsistentTheory consisT ∧ q ∈ maximalConsistentTheory consisT := by
+  have : maximalConsistentTheory consisT ⊢! p ⋏ q := mem_maximalConsistentTheory_iff.mp h
+  exact ⟨mem_maximalConsistentTheory_iff.mpr (by prover [this]),
+         mem_maximalConsistentTheory_iff.mpr (by prover [this])⟩
+
+lemma mem_maximalConsistentTheory_or {p q} (h : p ⋎ q ∈ maximalConsistentTheory consisT) :
+    p ∈ maximalConsistentTheory consisT ∨ q ∈ maximalConsistentTheory consisT := by
+  by_contra A
+  have b : maximalConsistentTheory consisT ⊢! ~p ∧ maximalConsistentTheory consisT ⊢! ~q := by
+    simpa [not_or, not_mem_maximalConsistentTheory_iff] using A
+  have : ¬Consistent (maximalConsistentTheory consisT) :=
+    inconsistent_of_provable (by prover [b.1, b.2, mem_maximalConsistentTheory_iff.mp h])
+  simp_all
+
+lemma maximalConsistentTheory_satisfiable :
+    (Formula.atom · ∈ maximalConsistentTheory consisT) ⊧* maximalConsistentTheory consisT := by
+  intro p hp
+  induction p using Formula.rec' <;> simp
+  case hatom => simpa
+  case hnatom =>
+    simpa using maximalConsistentTheory_consistent' hp
+  case hfalsum =>
+    have : ¬Consistent (maximalConsistentTheory consisT) := inconsistent_of_proof (axm hp)
+    simp_all
+  case hand p q ihp ihq =>
+    exact ⟨ihp (mem_maximalConsistentTheory_and hp).1, ihq (mem_maximalConsistentTheory_and hp).2⟩
+  case hor p q ihp ihq =>
+    rcases mem_maximalConsistentTheory_or hp with (hp | hq)
+    · left; exact ihp hp
+    · right; exact ihq hq
+
+lemma satisfiableTheory_of_consistent (consisT : Consistent T) : Semantics.SatisfiableTheory T :=
+  ⟨(Formula.atom · ∈ maximalConsistentTheory consisT),
+    Semantics.realizeTheory_of_subset maximalConsistentTheory_satisfiable (by simp)⟩
+
+theorem completeness! : T ⊨ p → T ⊢! p := by
+  suffices : Consistent (insert (~p) T) → Semantics.SatisfiableTheory (insert (~p) T)
+  · contrapose
+    simp; intro hp hs
+    have : Semantics.SatisfiableTheory (insert (~p) T) :=
+      this (consistent_insert_iff_not_refutable.mpr $ by simpa)
+    rcases this with ⟨v, hv⟩
+    have : v ⊧* T := Semantics.realizeTheory_of_subset hv (by simp)
+    have : v ⊧ p := hs this
+    have : ¬v ⊧ p := by simpa using hv (Set.mem_insert (~p) T)
+    contradiction
+  intro consis
+  exact satisfiableTheory_of_consistent consis
+
+noncomputable def completeness : T ⊨ p → T ⊢ p :=
+  λ h ↦ (completeness! h).toProof
+
+noncomputable instance : Complete (Formula α) where
+  complete := completeness
+
+end complete
+
+end Propositional
+
+end LO
